coq/Parser.v
@@ -7,6 +7,8 @@ Require Import GallStar.Termination.
 Import ListNotations.
 Open Scope list_scope.
 
+(* PARSER IMPLEMENTATION *)
+
 Record frame := Fr { loc : location
                    ; sem : forest
                    }.                               
@@ -15,6 +17,19 @@ Definition parser_stack := (frame * list frame)%type.
 
 Definition locStackOf (stk : parser_stack) : location_stack :=
   let (fr, frs) := stk in (fr.(loc), map loc frs).
+
+Fixpoint bottomFrame' (h : frame) (t : list frame) : frame :=
+  match t with
+  | []        => h
+  | fr :: frs => bottomFrame' fr frs
+  end.
+
+Definition bottomFrame (stk : parser_stack) : frame :=
+  let (h, t) := stk in bottomFrame' h t.
+
+Definition bottomFrameSyms (stk : parser_stack) : list symbol :=
+  let fr := bottomFrame stk
+  in  fr.(loc).(rpre) ++ fr.(loc).(rsuf).
   
 Record parser_state    := Pst { avail  : NtSet.t
                               ; stack  : parser_stack     
@@ -215,3 +230,202 @@ Definition mkInitState (g : grammar) (gamma : list symbol) (ts : list token) : p
 
 Definition parse (g : grammar) (gamma : list symbol) (ts : list token) : parse_result :=
   multistep g (mkInitState g gamma ts) (lex_nat_triple_wf _).
+
+(* PARSER-RELATED LEMMAS *)
+
+(* Lemmas for unfolding / inverting calls to step and multistep *)
+
+Lemma multistep_unfold :
+  forall g st a,
+    multistep g st a = 
+    match step g st as res return (step g st = res -> parse_result) with
+    | StepAccept sv => fun _  => Accept sv
+    | StepReject s  => fun _  => Reject s
+    | StepK st'     => fun hs =>
+                         multistep g st' (StepK_st_acc g st st' a hs)
+    | StepError s   => fun _  => Error s
+    end eq_refl.
+Proof.
+  intros; destruct a; auto.
+Qed.              
+
+Lemma multistep_cases' :
+  forall (g   : grammar)
+         (st  : parser_state)
+         (a   : Acc lex_nat_triple (meas g st))
+         (sr  : step_result)
+         (pr  : parse_result)
+         (heq : step g st = sr),
+    match sr as res return (step g st = res -> parse_result) with
+    | StepAccept sv => fun _ => Accept sv
+    | StepReject s => fun _  => Reject s
+    | StepK st' => fun hs => multistep g st' (StepK_st_acc g st st' a hs)
+    | StepError s => fun _ => Error s
+    end heq = pr
+    -> match pr with
+       | Accept f => sr = StepAccept f
+                     \/ exists st' a', sr = StepK st' 
+                                       /\ multistep g st' a' = Accept f
+       | Reject s => sr = StepReject s
+                     \/ exists st' a', sr = StepK st'
+                                       /\ multistep g st' a' = Reject s
+       | Error s  => sr = StepError s
+                     \/ exists st' a', sr = StepK st'
+                                       /\ multistep g st' a' = Error s
+       end.
+Proof.
+  intros g st a sr pr heq.
+  destruct pr; destruct sr; subst;
+    try solve [ intros; tc | intros h; inv h; auto | intros h; right; eauto ].
+Qed.
+
+Lemma multistep_cases :
+  forall (g : grammar)
+         (st : parser_state)
+         (a  : Acc lex_nat_triple (meas g st))
+         (pr  : parse_result),
+    multistep g st a = pr
+    -> match pr with
+       | Accept f => step g st = StepAccept f
+                     \/ exists st' a', step g st = StepK st' 
+                                       /\ multistep g st' a' = Accept f
+       | Reject s => step g st = StepReject s
+                     \/ exists st' a', step g st = StepK st'
+                                       /\ multistep g st' a' = Reject s
+       | Error s  => step g st = StepError s
+                     \/ exists st' a', step g st = StepK st'
+                                       /\ multistep g st' a' = Error s
+       end.
+Proof.
+  intros g st a pr hm; subst.
+  rewrite multistep_unfold.
+  eapply multistep_cases'; eauto.
+Qed.
+
+Lemma multistep_accept_cases :
+  forall (g : grammar)
+         (st : parser_state)
+         (a  : Acc lex_nat_triple (meas g st))
+         (f  : forest),
+    multistep g st a = Accept f
+    -> step g st = StepAccept f
+       \/ exists st' a', step g st = StepK st' 
+                         /\ multistep g st' a' = Accept f.
+Proof.
+  intros g st a f hm; subst.
+  destruct (multistep_cases g st a (Accept f)); auto.
+Qed.
+
+Lemma multistep_invalid_state_cases :
+  forall (g : grammar)
+         (st : parser_state)
+         (a  : Acc lex_nat_triple (meas g st)),
+    multistep g st a = Error InvalidState
+    -> step g st = StepError InvalidState
+       \/ exists st' a', step g st = StepK st' 
+                         /\ multistep g st' a' = Error InvalidState.
+Proof.
+  intros g st a hm; subst.
+  destruct (multistep_cases g st a (Error InvalidState)); auto.
+Qed.
+
+Lemma step_StepAccept_facts :
+  forall g av stk ts v,
+    step g (Pst av stk ts) = StepAccept v
+    -> (exists xo rpre v',
+           stk = (Fr (Loc xo rpre []) v', [])
+           /\ v' = v)
+       /\ ts = [].
+Proof.
+  intros g av stk ts v hs.
+  unfold step in hs; dms; tc.
+  inv hs; repeat eexists; eauto.
+Qed.
+
+(* A well-formedness invariant for the parser stack *)
+Inductive stack_wf (g : grammar) : parser_stack -> Prop :=
+| WF_nil :
+    forall pre suf v,
+      stack_wf g (Fr (Loc None pre suf) v, [])
+| WF_cons :
+    forall x xo' pre pre' suf suf' v v' frs,
+      In (x, pre ++ suf) g
+      -> stack_wf g (Fr (Loc xo' pre' (NT x :: suf')) v', frs) 
+      -> stack_wf g (Fr (Loc (Some x) pre suf) v, 
+                     Fr (Loc xo' pre' (NT x :: suf')) v' :: frs).
+
+Hint Constructors stack_wf.
+
+Lemma step_preserves_stack_wf_invar :
+  forall g av av' stk stk' ts ts',
+    step g (Pst av stk ts) = StepK (Pst av' stk' ts')
+    -> stack_wf g stk 
+    -> stack_wf g stk'.
+Proof.
+  intros g av av' stk stk' ts ts' hs hw.
+  unfold step in hs.
+  repeat (dmeq h); inv hs; tc.
+  - (* return *)
+    inv hw.
+    inv H10; constructor; auto.
+    rewrite <- app_assoc; auto.
+  - inv hw; auto.
+    constructor; auto.
+    rewrite <- app_assoc; auto.
+  - constructor; simpl; auto.
+    eapply llPredict_succ_arg_result_in_grammar; eauto.
+  - constructor; simpl; auto. 
+    eapply llPredict_ambig_arg_result_in_grammar; eauto.
+Qed.    
+
+(* The stack symbols that have already been processed represent
+   a (partial) derivation; this predicate relates those symbols
+   to the word (prefix) involved in the derivation. *)
+Inductive stack_derivation (g : grammar) : parser_stack -> list token -> Prop :=
+| SD_nil :
+    forall xo pre suf v w,
+      gamma_derivation g pre w v
+      -> stack_derivation g (Fr (Loc xo pre suf) v, []) w
+| SD_cons :
+    forall xo pre suf v fr' frs wpre wsuf,
+      gamma_derivation g pre wsuf v
+      -> stack_derivation g (fr', frs) wpre
+      -> stack_derivation g (Fr (Loc xo pre suf) v, fr' :: frs) (wpre ++ wsuf).
+
+Hint Constructors stack_derivation.
+
+(* tactic for inverting a stack_derivation hypothesis *)
+Ltac inv_sd hsd wpre wsuf hgd hsd' := inversion hsd as [? ? ? ? wpre hgd | ? ? ? ? ? ? wpre wsuf hgd hsd']; subst; clear hsd.
+
+(* Parser invariant: the processed stack symbols represent a 
+   partial derivation of a full word *)
+Inductive stack_derivation_invar (g : grammar) (stk : parser_stack) (wsuf w : list token) : Prop :=
+| SD_invar :
+    forall wpre,
+      stack_derivation g stk wpre
+      -> wpre ++ wsuf = w
+      -> stack_derivation_invar g stk wsuf w.
+
+(* Tactic for inverting a stack_derivation_invar hypothesis *)
+Ltac inv_sdi wpre hsd :=
+  match goal with
+  | H : stack_derivation_invar _ _ _ _ |- _ =>
+    inversion H as [wpre hsd ?]; subst; clear H
+  end.
+
+Lemma stack_derivation_cases :
+  forall g fr frs w,
+    stack_derivation g (fr, frs) w
+    -> match frs with
+       | []          => gamma_derivation g fr.(loc).(rpre) w fr.(sem)
+       | fr' :: frs' =>
+         exists wpre wsuf,
+         wpre ++ wsuf = w
+         /\ stack_derivation g (fr', frs') wpre
+         /\ gamma_derivation g fr.(loc).(rpre) wsuf fr.(sem)
+       end.
+Proof.
+  intros g fr frs w hsd.
+  destruct frs as [| fr' frs]; inv hsd; auto.
+  repeat eexists; repeat split; auto.
+Qed.
